examples/unit-tests/millionaires.fst
@@ -1,0 +1,94 @@
+module Wysteria
+open Prims.STATE
+
+type prin 
+type prins = set prin 
+type p_or_s = 
+  | Par 
+  | Sec
+type mode = { 
+  p_or_s: p_or_s; 
+  prins: prins 
+}
+assume (* private *) val moderef : ref mode
+
+kind Pre = mode => Type
+kind Post ('a:Type) = mode => 'a => mode => Type
+effect Wys ('a:Type) ('Pre:Pre) ('Post:Post 'a) =
+      ST 'a 
+         (fun h => 'Pre (SelHeap h moderef)) 
+         (fun h0 x h1 => 'Post (SelHeap h0 moderef) x (SelHeap h1 moderef))
+         (SomeRefs EmptySet)
+
+type Requires ('pre:Pre) = 'pre
+type Ensures : #'a:Type => Post 'a => Post 'a = fun ('a:Type) ('post:Post 'a) => 'post
+
+assume val get_mode : unit -> Wys mode
+                           (Requires (fun h => True)) 
+                           (Ensures mode (fun m0 r m1 => m0==m1 /\ r==m1))
+
+(* private  *)
+assume val set_mode : m:mode -> Wys unit
+                             (Requires (fun h => True))
+                             (Ensures unit (fun m0 r m1 => m1==m))
+                           
+let with_mode ('a:Type) ('Pre:Pre) ('Post:Post 'a) (m:mode) (f:unit -> Wys 'a 'Pre 'Post) =
+  let cur = get_mode () in
+  (match cur.p_or_s with 
+   | Sec -> assert (cur.prins == m.prins)
+   | Par -> assert (SubsetEq prin cur.prins m.prins));
+  set_mode m;
+  let res = f () in 
+  set_mode cur;
+  res
+           
+type box 'a = 
+  | Box : v:'a -> m:mode -> box 'a
+
+let mk_box (x:'a) (u:unit) = Box x (get_mode())
+
+let unbox (x:box 'a) (u:unit) = 
+  let cur = get_mode () in
+  assert (SupsetEq prin (Box.m x).prins cur.prins);
+  Box.v x
+
+type wire 'a = PartialMap.t prin 'a
+open PartialMap
+ 
+let mk_wire (m:mode) (x:box 'a) = 
+  let f (u:unit) = ConstMap m.prins (unbox x ()) in
+  match m.p_or_s with 
+  | Sec -> f ()
+  | Par -> with_mode m f
+
+let concat_wires (w1:wire 'a) (w2:wire 'a) = 
+  assert (DisjointDom prin 'a w1 w2);
+  Concat w1 w2
+
+let project_wire (w:wire 'a) (p:prin) = 
+  assert (InDom p w);
+  let cur = get_mode () in
+  (match cur.p_or_s with 
+   | Sec -> assert (InSet p cur.prins)
+   | Par -> assert (SetEqual cur.prins (Singleton p)));
+  Sel w p
+                                
+(* -------------------------------------------------------------------------------- *)
+
+module Millionaires
+open Wysteria
+assume val A : prin
+assume val B : prin
+assume AB_distinct: A=!=B
+
+val is_A_richer_than_B : unit -> Wys bool
+                                     (Requires (fun m => m.p_or_s==Par /\ SetEqual m.prins EmptySet))// (Singleton prin A)))// (Union (Singleton A) (Singleton B))))
+                                     (Ensures bool (fun m0 res m1 => res == false))
+let is_A_richer_than_B (u:unit) = 
+  let par_A = {p_or_s=Par; prins=Singleton A} in
+  let par_B = {p_or_s=Par; prins=Singleton B} in
+  let sec_AB = {p_or_s=Sec; prins=Union (Singleton A) (Singleton B)} in
+  let x = with_mode par_A (mk_box 2) in
+  let y = with_mode par_B (mk_box 3) in
+  let z = concat_wires (mk_wire par_A x) (mk_wire par_B y) in
+  with_mode sec_AB (fun (u:unit) -> project_wire z A > project_wire z B)
